doc/simple/coq/Subst.v
@@ -1,0 +1,77 @@
+Require Import CtxExtension.
+Require Import LibLN.
+Require Import AlgoDef.
+Require Import UtilityEnv.
+Require Import DeclDef.
+
+Lemma ctxsubst_inv_empty : forall I,
+    ACpltCtxSubstCtx empty empty I ->
+    I = empty.
+Proof.
+  intros. inversions H; auto.
+  false. apply* empty_push_inv.
+  false. apply* empty_push_inv.
+  false. apply* empty_push_inv.
+  false. apply* empty_push_inv.
+  false. apply* empty_push_inv.
+  false. apply* empty_push_inv.
+Qed.
+
+Lemma ctxsubst_inv_var : forall H G I x,
+    ACpltCtxSubstCtx (H & x ~ AC_Var) (G & x ~ AC_Var) I ->
+    CompleteCtx H /\
+    ACpltCtxSubstCtx H G I.
+Proof.
+  intros. inversions H0.
+  false. apply* empty_push_inv.
+  destruct (eq_push_inv H2) as [? [? ?]]; subst.
+  destruct (eq_push_inv H3) as [? [? ?]]; subst.
+  auto.
+  destruct (eq_push_inv H2) as [? [? ?]].
+  false.
+  destruct (eq_push_inv H2) as [? [? ?]].
+  false.
+  destruct (eq_push_inv H2) as [? [? ?]].
+  false.
+  destruct (eq_push_inv H2) as [? [? ?]].
+  false.
+  destruct (eq_push_inv H2) as [? [? ?]].
+  false.
+Qed.
+
+Lemma ctxsubst_inv_typvar : forall H G I' x t1 t2,
+    ACpltCtxSubstCtx (H & x ~ AC_Typ t1) (G & x ~ AC_Typ t2) I' ->
+    exists I t1', (I' = I & x ~ DC_Typ t1' /\
+    CompleteCtx H /\ ACpltCtxSubstCtx H G I /\ ACtxSubst H t1 = ACtxSubst H t2 /\
+    ACpltCtxSubst H t1 t1').
+Proof.
+  intros. inversions H0.
+  false. apply* empty_push_inv.
+  destruct (eq_push_inv H2) as [? [? ?]]. false.
+  exists I t1'.
+  destruct (eq_push_inv H2) as [? [? ?]]; subst.
+  destruct (eq_push_inv H3) as [? [? ?]]; subst.
+  inversions H8; inversions H1.
+  auto.
+  destruct (eq_push_inv H2) as [? [? ?]]. false.
+  destruct (eq_push_inv H2) as [? [? ?]]. false.
+  destruct (eq_push_inv H2) as [? [? ?]]. false.
+  destruct (eq_push_inv H2) as [? [? ?]]. false.
+Qed.
+
+Lemma stable_cplt_env : forall G H I J,
+    ExtCtx G H ->
+    ACpltCtxSubstCtx H G I ->
+    ACpltCtxSubstCtx H H J ->
+    I = J.
+Proof.
+  intros. inductions H0.
+  pose (ctxsubst_inv_empty I H1).
+  pose (ctxsubst_inv_empty J H2).
+  rewrite e. rewrite e0. auto.
+  destruct (ctxsubst_inv_var H G I x H3) as [_ ?].
+  destruct (ctxsubst_inv_var H H J x H4) as [_ ?].
+  apply* IHExtCtx.
+  destruct (ctxsubst_inv_typvar H G I x t2 t1 H4) as [I1' [t1' [? [_ [? ?]]]]].
+Admitted.
+  
